examples/refcounter2/Frac.s.dfy
@@ -3,6 +3,7 @@ include "Rational.s.dfy"
 module FracLogic {
   import opened Rationals
 
+  // TODO user should not be able to construct this
   linear datatype Frac<V> = Frac(linear v: V, r: PositiveRational)
 
   function method {:extern} borrow<V>(shared frac: Frac<V>) : (shared v : V)
@@ -15,12 +16,12 @@ module FracLogic {
   function method {:extern} wrap<V>(linear v: V) : (linear frac : Frac<V>)
   ensures frac == Frac(v, one())
 
-  function method {:extern} frac_split<V>(
+  method {:extern} frac_split<V>(
       linear f: Frac<V>,
       ghost r: PositiveRational)
-    : (linear res: (Frac<V>, Frac<V>))
+  returns (linear a: Frac<V>, linear b: Frac<V>)
   requires Rationals.lt(r, f.r)
-  ensures res.0 == Frac(f.v, r)
-  ensures res.1 == Frac(f.v, Rationals.minus(f.r, r))
+  ensures a == Frac(f.v, r)
+  ensures b == Frac(f.v, Rationals.minus(f.r, r))
 
 }
